src/cbor/pulse/raw/everparse/CBOR.Pulse.Raw.EverParse.Det.Serialize.fsti
@@ -16,12 +16,18 @@ module U64 = FStar.UInt64
    ============================================================ *)
 
 noextract [@@noextract_to "krml"]
-val cbor_serialize_tag_postcond
+let cbor_serialize_tag_postcond
   (tag: raw_uint64)
   (output: S.slice U8.t)
   (res: SZ.t)
   (v': Seq.seq U8.t)
 : Tot prop
+= let s = serialize_cbor_tag tag in
+  let len = Seq.length s in
+  SZ.v (S.len output) == Seq.length v' /\
+  SZ.v res <= Seq.length v' /\
+  (res == 0sz <==> len > Seq.length v') /\
+  (len <= Seq.length v' ==> Seq.slice v' 0 (SZ.v res) == s)
 
 val cbor_serialize_array_precond
   (len: raw_uint64)
